Schema.v
@@ -1,3 +1,4 @@
+Require Export Coq.Sets.Multiset.
 Require Import SfLib.
 
 
@@ -25,3 +26,26 @@ Inductive schema_column_has_type: schema_ty -> col -> col_ty -> Prop :=
       i = S(i') ->
       s = c' *** s' ->
       schema_column_has_type s' i c'.
+
+
+(* The type of each tuple within a relation with the given schema. *)
+Fixpoint support (s: schema_ty) : Type :=
+  match s with
+  | STyNil => unit
+  | a *** => helper a
+  | a *** s' => (helper a) * support s'
+  end
+with helper(c: col_ty) : Type :=
+  match c with
+  | CTyNat => nat
+  | CTyBag s_nested => multiset (support s_nested)
+  end.
+
+
+(* Construct a custom equality function over the support of s. *)
+Definition support_eq (s: schema_ty) (row1 row2: support s) : Prop := (row1 = row2).
+
+Lemma support_eq_dec (s: schema_ty):
+  forall (x y : support s), {(support_eq s) x y} + {~ (support_eq s) x y}.
+Proof.
+  intros. unfold support_eq. Admitted.
