Mapping.v
@@ -1,8 +1,14 @@
 Require Export Pig.Relations.
 
+
 Definition mapper (s s': schema_ty) : Type := (support s) -> (support s').
+
 
 Inductive mapped (s s': schema_ty) : relation s -> mapper s s' -> relation s' -> Prop :=
 | Mapped: forall (r: relation s) (m: mapper s s') (r': relation s'),
     (* TODO: Add constraints. *)
     mapped s s' r m r'.
+
+
+(* These examples build on the examples in `Relations`. *)
+Example nat_identity_mapper := fun (n: nat) => n.
